\documentclass[UTF8]{ctexart}
    \title{算法分析与设计基础作业2}
    \author{软件71 骆炳君 2017013573}
    \date{\today}
\usepackage{amsmath}
\usepackage{amssymb}
\allowdisplaybreaks[1]
\begin{document}
\maketitle
\pagenumbering{arabic}

\paragraph{1.}
\subparagraph{a.}
\begin{align*}
    &\text{设}m=lgn,\text{则}T(2^m)=2T(2^{m/2})+1\\
    &\text{设}S(m)=T(2^m),\text{则}S(m)=2S(m/2)+1\\
    &\because f(m)=1=O(m^{log_22-\epsilon})\\
    &\therefore S(m)=\Theta(m^{log_22})=\Theta(m)\\
    &\therefore T(n)=S(m)=\Theta(lgn)
\end{align*}

\subparagraph{b.}
\begin{align*}
    &\because nT(n)=(n-2)T(n-1)+2\\
    &
    \begin{aligned}
        \therefore T(n)&=\frac{n-2}{n}T(n-1)+\frac{2}{n}\\
        &=\frac{n-2}{n}(\frac{n-3}{n-1}T(n-2)+\frac{2}{n})+\frac{2}{n}\\
        &=\frac{2}{n(n-1)}T(2)+\frac{2}{n}\sum_{k=1}^{n}\frac{k(k-1)}{n(n-1)}\\
        &=\Theta(1)
    \end{aligned}
\end{align*}

\end{document}