---
  output:
    pdf_document: default
    html_document: default
---
# Homework 8
Luo Bingjun 2017013573 Software 71
2019/5/23

## Prob-1: KNNL 7.33
$$
\begin{aligned}
SSR(X_1)&=\sum(b_1(X_1-\bar{X_1}))^2\\
&=\frac{b_1^2(\sum(X_1-\bar{X_1})^2)^2}{\sum(X_1-\bar{X_1})^2}\\
&=\frac{(\sum(X_1-\bar{X_1}(Y-\bar{Y})^2)^2}{\sum(X_1-\bar{X_1})^2}\\
&=r_{Y1}^2\sum(Y-\bar{Y})^2
\end{aligned}
$$

$$
SSE(X_1)=SST-SSR(X_1)=(1-r_{Y1}^2)\sum(Y-\bar{Y})^2
$$

$$
SSR(X_1,X_2)=b_1\sum(X_1-\bar{X_1})(Y-\bar{Y})+b_2\sum(X_2-\bar{X_2})(Y-\bar{Y})
$$

From (7.56) we can obtain
$$
SSR(X_1,X_2)=\frac{1}{1-r_{12}^2}((r_{Y1}^2+r_{Y2}^2)\sum(Y-\bar{Y})^2+2r_{Y1}r_{Y2}r_{12}\sum(Y-\bar{Y})^2)
$$

$$
\begin{aligned}
r_{Y2|1}^2&=\frac{SSR(X_1,X_2)-SSR(X_1)}{SSE(X_1)}\\
&=\frac{(r_{Y1}^2+r_{Y2}^2+2r_{Y1}r_{Y2}r_{12}-r_{Y1}^2(1-r_{12}^2))\sum(Y-\bar{Y})^2}{(1-r_{Y1}^2)(1-r_{12}^2)\sum(Y-\bar{Y})^2}\\
&=\frac{(r_{Y2}-r_{12}r_{Y1})^2}{(1-r_{Y1}^2)(1-r_{12}^2)}
\end{aligned}
$$